\documentclass[14pt,fleqn]{extarticle}
\RequirePackage{prepwell}

\previewoff 

\newcommand\fa{x^{\sin x}}
\newcommand\sa{\left(\sin x \right)^{\cos x}}

\begin{document} 

Differentiate the following 
\[ \qquad x^{\sin x} + \left(\sin x \right)^{\cos x} \] 

\newcard 

\begin{align}
	y &= \underbrace{\fa}_A + \underbrace{\sa}_B \\
	\therefore \log y &= \log A + \log B  \\
	\implies \frac{d}{dx}\log y &= \frac{d}{dx}\log A + \frac{d}{dx}\log B \\
	\text{where } \frac{d}{dx}\log y &= \frac{1}{y}\cdot \frac{dy}{dx}
\end{align}

And this is how we will find $\frac{dy}{dx}$ 

\newcard 

If $y = A + B$, then $\frac{dy}{dx} = \frac{dA}{dx} + \frac{dB}{dx}$ \newline 

But it does \underline{not} mean that 
\[ \qquad \log y = \log A + \log B \] 

\newcard 

\begin{align}
	A &= \fa \implies \log A = \sin x\cdot \left(\log x \right) \\
	\therefore \frac{1}{A} \frac{dA}{dx} &= \left[\frac{\sin x}{x} + \left(\log x \right)\cdot \cos x  \right] \\
	\implies \frac{dA}{dx} &= \fa \left[\frac{\sin x}{x} + \log \left(x^{\cos x} \right)\right]
\end{align}

\newcard 

\begin{align}
	A &= \fa \implies \frac{dA}{dx} = x^{ \sin x - 1} 
\end{align}

\newcard 

$\dfrac{d}{dx}x^n = n\cdot x^{n-1}$ is true \underline{only when} $n$ is a constant. If it is anything else, then we must look at taking $\log$. Which is why 

\begin{align}
	A &= \fa \implies \log A = \sin x\cdot \left(\log x \right) \\
	\therefore \frac{1}{A} \frac{dA}{dx} &= \left[\frac{\sin x}{x} + \left(\log x \right)\cdot \cos x  \right] \\
	\implies \frac{dA}{dx} &= \underbrace{\fa \left[\frac{\sin x}{x} + \log \left(x^{\cos x} \right)\right]}_{b\cdot \log a = \log \left(a^b \right)}
	\end{align} 
	
	\newcard 
	
	Similarly 
	\[ \frac{dB}{dx} = \sa \left[\frac{\cos^2 x}{\sin x} - \log \left(\sin x \right)^{\sin x} \right]\] 
	
	And hence 
	\begin{align}
	\frac{dy}{dx} &= \fa \left[\frac{\sin x}{x} + \log \left(x^{\cos x} \right)\right] \\
	&+ \sa \left[\frac{\cos^2 x}{\sin x} - \log \left(\sin x \right)^{\sin x} \right]
\end{align}
	
	\newcard 
	
	\begin{align}
	   B &= \sa \implies \log B = \cos x\cdot \left(\log \sin x \right) \\
	   \therefore \frac{1}{B}\frac{dB}{dx} &= \left[\cos x \frac{d}{dx} \left(\log\sin x \right) + \left(\log \sin x \right)\cdot \frac{d}{dx}\cos x  \right] \\
	   &= \left[\frac{\cos x}{\sin x}\cdot \cos x - \left(\log \sin x \right)\sin x \right] \\
	   &= \left[\frac{\cos^2 x}{\sin x} - \log \left(\sin x \right)^{\sin x}\right] \\
	   \therefore \frac{dB}{dx} &= \sa \left[\frac{\cos^2 x}{\sin x} - \log \left(\sin x \right)^{\sin x}\right] \\
	   \text{and } \frac{dy}{dx} &= \overbrace{\fa \left[\frac{\sin x}{x} + \log \left(x^{\cos x} \right)\right]}^{\frac{dA}{dx}} \\
	&+ \underbrace{\sa \left[\frac{\cos^2 x}{\sin x} - \log \left(\sin x \right)^{\sin x} \right]}_{\frac{dB}{dx}}
\end{align}
\end{document} 
